theories/L2_typeStripped/term.v
@@ -67,7 +67,7 @@ Fixpoint print_term (t:Term) : string :=
   match t with
     | TRel n => "(Rel " ++ (nat_to_string n) ++ ")"
     | TSort _ => " SRT "
-    | TProof => " PRF "
+    | TProof t => "(PRF " ++ print_term t ++ ")"
     | TCast t  => "(CAST " ++ print_term t ++ ")"
     | TProd nm t => "(PROD "++ (print_name nm) ++ " [" ++ print_term t ++ "])"
     | TLambda nm t => "(LAM "++ (print_name nm) ++ " [" ++ print_term t ++ "])"
@@ -98,9 +98,10 @@ Proof.
   apply TrmTrmsDefs_ind.
   - induction t; cross. destruct (eq_nat_dec n n0); [lft | rght].
   - induction t; cross. destruct (Srt_dec s s0); [lft | rght].
-  - induction t; cross. intuition.
   - induction t0; cross.
-    destruct (H t0); [lft | rght ..]. 
+    destruct (H t0); [lft | rght ..].
+  - induction t0; cross.
+    destruct (H t0); [lft | rght ..].
   - induction t0; cross.
     destruct (name_dec n n0); destruct (H t0); [lft | rght ..]. 
   - induction t0; cross.
@@ -230,33 +231,6 @@ Proof.
   try (right; intros h; destruct h as [x0 [x1 [x2 j]]]; discriminate).
   - left. auto.
 Qed.
-
-Function isL2Cnstr (t:Term) : option (inductive * nat * nat) :=
-  match t with
-    | TConstruct i cn arty => Some (i, cn, arty)
-    | TCast u => isL2Cnstr u
-    | _ => None
-  end.
-
-Lemma isL2Cnstr_spec:
-  forall t i cn arty,
-    isL2Cnstr t = Some (i, cn, arty) ->
-    (t = TConstruct i cn arty) \/
-    exists u, (t = TCast u /\ isL2Cnstr u = Some (i, cn, arty)).
-Proof.
-  induction t; intros; cbn in H; try discriminate.
-  - destruct (IHt _ _ _ H).
-    + right. exists t. intuition.
-    + right. exists t. intuition.
-  - myInjection H. left. reflexivity.
-Qed.
-
-Function isL2Rel (t:Term) : option nat :=
-  match t with
-    | TRel n => Some n
-    | TCast u => isL2Rel u
-    | _ => None
-  end.
 
 Inductive isCanonical : Term -> Prop :=
 | canC: forall (i:inductive) (n m:nat), isCanonical (TConstruct i n m)
@@ -617,26 +591,6 @@ induction t; intros arg args h; simpl; try reflexivity.
 - elim h. exists t1, t2, t3. reflexivity.
 Qed.
 
-Lemma isL2Cnstr_mkApp_Some:
-  forall t ts i x arty,
-    isL2Cnstr (mkApp t ts) = Some (i, x, arty) ->
-    ts = tnil \/ isL2Cnstr t = Some (i, x, arty).
-Proof.
-  intros. functional induction (mkApp t ts).
-  - cbn in H. discriminate.
-  - right. assumption.
-  - cbn in H. discriminate.
-Qed.
-
-Lemma isL2Cnstr_mkApp_None:
-    forall t u us,
-    isL2Cnstr t = None -> isL2Cnstr (mkApp t (tcons u us)) = None.
-Proof.
-  intros. case_eq (isL2Cnstr (mkApp t (tcons u us))); intros.
-  - assert (j:= mkApp_isApp t u us).
-    destruct j as [x0 [x1 [x2 k]]]. rewrite k in H0. cbn in H0. discriminate.
-  - reflexivity.
-Qed.  
 
 (** main lemma for dealing with mkApp **)
 Lemma mkApp_isApp_lem:
@@ -650,8 +604,8 @@ Proof.
     left. intuition. revert H. not_isApp.
   - exists (TSort s), arg, tnil. split. reflexivity.
     left. intuition. revert H. not_isApp.
-  - exists TProof, arg, tnil. split. reflexivity.
-    left. intuition. revert H. not_isApp.
+  - exists (TProof fn), arg, tnil. split. reflexivity.
+    + left. intuition. revert H. not_isApp. 
   - exists (TCast fn), arg, tnil. split. reflexivity.
     + left. intuition. revert H. not_isApp. 
   - exists (TProd n fn), arg, tnil. split. reflexivity.
@@ -694,8 +648,8 @@ Qed.
 Inductive WFapp: Term -> Prop :=
 | wfaRel: forall m, WFapp (TRel m)
 | wfaSort: forall srt, WFapp (TSort srt)
-| wfaPrf: WFapp TProof
 | wfaCast: forall tm, WFapp tm -> WFapp (TCast tm)
+| wfaProof: forall tm, WFapp tm -> WFapp (TProof tm)
 | wfaProd: forall nm bod, WFapp bod -> WFapp (TProd nm bod)
 | wfaLambda: forall nm bod, WFapp bod -> WFapp (TLambda nm bod)
 | wfaLetIn: forall nm dfn bod,
@@ -825,8 +779,8 @@ Qed.
 Inductive WFTrm: Term -> nat -> Prop :=
 | wfRel: forall n m, m < n -> WFTrm (TRel m) n
 | wfSort: forall n s, WFTrm (TSort s) n
-| wfPrf: forall n, WFTrm TProof n
 | wfCast: forall n t, WFTrm t n -> WFTrm (TCast t) n
+| wfProof: forall n t, WFTrm t n -> WFTrm (TProof t) n
 | wfProd: forall n nm bod,
             WFTrm bod (S n) -> WFTrm (TProd nm bod) n
 | wfLambda: forall n nm bod,
@@ -879,6 +833,7 @@ Inductive PoccTrm : Term -> Prop :=
 | PoProdBod: forall s bod, PoccTrm bod -> PoccTrm (TProd s bod)
 | PoLambdaBod: forall s bod, PoccTrm bod -> PoccTrm (TLambda s bod)
 | PoCast: forall t, PoccTrm t -> PoccTrm (TCast t)
+| PoProof: forall t, PoccTrm t -> PoccTrm (TProof t)
 | PoLetInDfn: forall s dfn bod,
                 PoccTrm dfn -> PoccTrm (TLetIn s dfn bod)
 | PoLetInBod: forall s dfn bod,
@@ -1102,6 +1057,9 @@ Proof.
   - destruct args; simpl.
     + apply PoCast. assumption.
     + apply PoAppL. apply PoCast. assumption.
+  - destruct args; simpl.
+    + apply PoProof. assumption.
+    + apply PoAppL. apply PoProof. assumption.
  - destruct args; simpl.
     + apply PoLetInDfn. assumption.
     + apply PoAppL. apply PoLetInDfn. assumption.
@@ -1161,9 +1119,10 @@ Inductive Instantiate: nat -> Term -> Term -> Prop :=
 | IRelGt: forall n m, n > m -> Instantiate n (TRel m) (TRel m)
 | IRelLt: forall n m, n < m -> Instantiate n (TRel m) (TRel (pred m))
 | ISort: forall n srt, Instantiate n (TSort srt) (TSort srt)
-| IProof: forall n, Instantiate n TProof TProof
 | ICast: forall n t it,
-           Instantiate n t it -> Instantiate n (TCast t) it
+           Instantiate n t it -> Instantiate n (TCast t) (TCast it)
+| IProof: forall n t it,
+           Instantiate n t it -> Instantiate n (TProof t) (TProof it)
 | IProd: forall n nm bod ibod,
              Instantiate (S n) bod ibod -> 
              Instantiate n (TProd nm bod) (TProd nm ibod)
@@ -1221,31 +1180,36 @@ Lemma Instantiates_no_gen:
   (forall n t s, Instantiate n t s -> PoccTrm s -> PoccTrm t) /\
   (forall n ts ss, Instantiates n ts ss -> PoccTrms ss -> PoccTrms ts) /\
   (forall n ds es, InstantiateDefs n ds es -> PoccDefs es -> PoccDefs ds).
-intro h. apply InstInstsDefs_ind; intros; auto.
-- destruct (Pocc_mkApp_inv _ _ H). 
-  + contradiction.
-  + inversion H0.
-- inversion H.
-- inversion_Clear H0.
-  + constructor. intuition. 
-- inversion_Clear H0.
-  + constructor. intuition. 
-- inversion_Clear H1.
-  + constructor. intuition. 
-  + apply PoLetInBod. intuition.
-- destruct (Pocc_mkApp_inv _ _ H2) as [hit | hiats]; intuition.
-  inversion hiats; intuition.
-- inversion_Clear H1.
-  + constructor. intuition.
-  + apply PoCaseR. intuition.
-- inversion_Clear H0.
-  + constructor. apply H. assumption.
-- inversion_Clear H1.
-  + constructor. intuition.
-  + apply PoTtl. intuition.
-- inversion_Clear H1.
-  + constructor. intuition. 
-  + apply PoDtl. intuition. 
+Proof.
+  intro h. apply InstInstsDefs_ind; intros; auto.
+  - destruct (Pocc_mkApp_inv _ _ H). 
+    + contradiction.
+    + inversion H0.
+  - inversion H.
+  - inversion_Clear H0.
+    + constructor. intuition.
+  - inversion_Clear H0.
+    + constructor. intuition.
+  - inversion_Clear H0.
+    + constructor. intuition. 
+  - inversion_Clear H0.
+    + constructor. intuition. 
+  - inversion_Clear H1.
+    + constructor. intuition. 
+    + apply PoLetInBod. intuition.
+  - destruct (Pocc_mkApp_inv _ _ H2) as [hit | hiats]; intuition.
+    inversion hiats; intuition.
+  - inversion_Clear H1.
+    + constructor. intuition.
+    + apply PoCaseR. intuition.
+  - inversion_Clear H0.
+    + constructor. apply H. assumption.
+  - inversion_Clear H1.
+    + constructor. intuition.
+    + apply PoTtl. intuition.
+  - inversion_Clear H1.
+    + constructor. intuition. 
+    + apply PoDtl. intuition. 
 Qed.
 
 Function instantiate (n:nat) (tbod:Term) {struct tbod} : Term :=
@@ -1265,7 +1229,8 @@ Function instantiate (n:nat) (tbod:Term) {struct tbod} : Term :=
     | TLetIn nm tdef bod =>
       TLetIn nm (instantiate n tdef) (instantiate (S n) bod)
     | TFix ds m => TFix (instantiateDefs (n + dlength ds) ds) m
-    | TCast t => instantiate n t
+    | TCast t => TCast (instantiate n t)
+    | TProof t => TProof (instantiate n t)
     | x => x
   end
 with instantiates (n:nat) (args:Terms) {struct args} : Terms :=
@@ -1330,21 +1295,14 @@ Lemma instantiate_Instantiate:
   (forall t n, Instantiate n t (instantiate n t)) /\
   (forall ts n, Instantiates n ts (instantiates n ts)) /\
   (forall (ds:Defs) n, InstantiateDefs n ds (instantiateDefs n ds)).
-apply TrmTrmsDefs_ind; intros; simpl; try (solve [constructor]).
-- destruct (lt_eq_lt_dec n0 n) as [[h | h] | h].
-  + rewrite (proj1 (nat_compare_lt _ _) h). apply IRelLt. assumption.
-  + rewrite (proj2 (nat_compare_eq_iff _ _) h). subst. apply IRelEq.
-  + rewrite (proj1 (nat_compare_gt _ _)). apply IRelGt.
-    assumption. assumption.
-- apply ICast;intuition.
-- apply IProd; intuition.
-- apply ILambda; intuition.
-- apply ILetIn; intuition.
-- apply IApp; intuition.
-- apply ICase; intuition.
-- apply IFix; intuition.
-- apply Icons; intuition.
-- apply Idcons; intuition.
+Proof.
+  apply TrmTrmsDefs_ind; intros; simpl; try (solve [constructor]);
+  try (solve[constructor; intuition]).
+  - destruct (lt_eq_lt_dec n0 n) as [[h | h] | h].
+    + rewrite (proj1 (nat_compare_lt _ _) h). apply IRelLt. assumption.
+    + rewrite (proj2 (nat_compare_eq_iff _ _) h). subst. apply IRelEq.
+    + rewrite (proj1 (nat_compare_gt _ _)). apply IRelGt.
+      assumption. assumption.
 Qed.
 
 Lemma instant_pres_PoccTrm:
@@ -1353,7 +1311,6 @@ Lemma instant_pres_PoccTrm:
   (forall (Ds:Defs), PoccDefs Ds -> forall n, PoccDefs (instantiateDefs n Ds)).
 Proof.
   apply poTrmTrmsDefs_ind; intros; cbn; try solve [constructor; trivial].
-  - apply H0.
   - eapply Pocc_TApp_mkApp. apply PoAppL. auto.
   - eapply Pocc_TApp_mkApp. apply PoAppA. auto.
   - eapply Pocc_TApp_mkApp. apply PoAppR. auto.
@@ -1406,8 +1363,8 @@ Proof.
     + rewrite (proj1 (nat_compare_lt _ _) h). constructor.
     + rewrite (proj2 (nat_compare_eq_iff _ _) h). apply mkApp_pres_WFapp; auto.
     + rewrite (proj1 (nat_compare_gt _ _) h). constructor.
-  - change (WFapp (instantiate t n tm)). 
-    + apply H0. assumption.
+  - cbn. constructor. apply H0. assumption.
+  - cbn. constructor. apply H0. assumption.
   - change (WFapp (TProd nm (instantiate t (S n) bod))).
     constructor.
     + apply H0. assumption.
